Trail.v
@@ -1,0 +1,225 @@
+Require Export SystemFR.ErasedQuant.
+
+Opaque reducible_values.
+
+(** This file specifies with axioms a model for updates and lookups in trails *)
+
+(** We assume that we have a type `T_tree` that represents a tree of values, together with *)
+(** an encoding of their types *)
+Parameter T_tree: tree.
+Axiom tree_fv: forall tag, pfv T_tree tag = nil.
+Axiom wf_tree: wf T_tree 0.
+Axiom is_erased_type_tree: is_erased_type T_tree.
+Hint Resolve tree_fv: fv.
+Hint Resolve wf_tree: wf.
+Hint Resolve is_erased_type_tree: erased.
+
+(* We assume we have an empty tree *)
+Parameter empty_tree: tree.
+Axiom empty_tree_type: [ empty_tree : T_tree ]v.
+
+(** We consider a type `T_key` that represents a sequence of selections in a tree *)
+Parameter T_key: tree.
+Axiom key_fv: forall tag, pfv T_key tag = nil.
+Axiom wf_key: wf T_key 0.
+Axiom is_erased_type_key: is_erased_type T_key.
+Hint Resolve key_fv: fv.
+Hint Resolve wf_key: wf.
+Hint Resolve is_erased_type_key: erased.
+
+(** These types have no free variables, so substitutions keep them unchanged *)
+Lemma substitute_tree:
+  forall l tag, psubstitute T_tree l tag = T_tree.
+Proof.
+  intros; apply substitute_nothing5; eauto using tree_fv.
+Qed.
+
+Lemma substitute_key:
+  forall l tag, psubstitute T_key l tag = T_key.
+Proof.
+  intros; apply substitute_nothing5; eauto using key_fv.
+Qed.
+
+(** We consider a `tlookup` function that for a type `A` and a tree `t` looks up a value at the *)
+(** root of the tree. If the tag at the root corresponds to type `A`, it returns the value at the *)
+(** root. Otherwise, it returns the empty list `tnil` or `tleft uu`. We assume that the type *)
+(** `A` that appears in `tlookup` contain the empty list, which is the case for the types `T_top` *)
+(** and `List` presented in the paper.  *)
+(** tlookup: (A: type) -> T_tree -> A *)
+Parameter tlookup: tree -> tree -> tree.
+
+Axiom open_lookup:
+  forall k A t rep,
+    open k (tlookup A t) rep = tlookup (open k A rep) (open k t rep).
+
+Axiom substitute_lookup:
+  forall A t l tag,
+    psubstitute (tlookup A t) l tag =
+    tlookup (psubstitute A l tag) (psubstitute t l tag).
+
+Axiom wf_lookup:
+  forall k A t,
+    wf A k ->
+    wf t k ->
+    wf (tlookup A t) k.
+Hint Resolve wf_lookup: wf.
+
+Axiom is_erased_term_lookup:
+  forall A t,
+    is_erased_type A ->
+    is_erased_term t ->
+    is_erased_term (tlookup A t).
+Hint Resolve is_erased_term_lookup: erased.
+
+Axiom lookup_type:
+  forall A tree,
+    [ tleft uu : A ]v ->
+    [ tree : T_tree ]v ->
+    [ tlookup A tree : A ].
+
+Axiom lookup_onto:
+  forall a A,
+    [ a : A ]v ->
+    exists tree,
+      [ tree : T_tree ]v /\
+      [ tlookup A tree ≡ a ].
+
+Axiom lookup_fv:
+  forall A trail tag,
+    pfv (tlookup A trail) tag = pfv A tag ++ pfv trail tag.
+
+(** We also assume we have a function `select`, that uses a sequence of selections to select a *)
+(** subtree of a tree *)
+(** select: T_key -> T_tree -> T_tree *)
+Parameter select: tree -> tree -> tree.
+
+Axiom select_type:
+  forall key tree,
+    [ key : T_key ]v ->
+    [ tree : T_tree ]v ->
+    [ select key tree : T_tree ]v.
+
+Axiom evaluate_select:
+  forall key trail1 trail2,
+    star scbv_step trail1 trail2 ->
+    star scbv_step (select key trail1) (select key trail2).
+
+Axiom wf_select:
+  forall k t1 t2,
+    wf t1 k ->
+    wf t2 k ->
+    wf (select t1 t2) k.
+
+Axiom psubstitute_select:
+  forall t1 t2 l tag,
+    psubstitute (select t1 t2) l tag =
+    select (psubstitute t1 l tag) (psubstitute t2 l tag).
+
+Axiom open_select:
+  forall k t1 t2 rep,
+    open k (select t1 t2) rep =
+    select (open k t1 rep) (open k t2 rep).
+
+Axiom pfv_select:
+  forall t1 t2 tag, pfv (select t1 t2) tag = pfv t1 tag ++ pfv t2 tag.
+
+Axiom is_erased_term_select:
+  forall t1 t2,
+    is_erased_term t1 ->
+    is_erased_term t2 ->
+    is_erased_term (select t1 t2).
+
+Hint Resolve wf_select: wf.
+Hint Resolve is_erased_term_select: erased.
+
+Lemma open_tdots:
+  forall Γ key tree,
+    [ key : T_key ]v ->
+    [ Γ ⊨ tree : T_tree ] ->
+    [ Γ ⊨ select key tree : T_tree ].
+Proof.
+  unfold open_reducible;
+    repeat step || rewrite psubstitute_select ||
+           t_instantiate_sat3_nil || rewrite substitute_tree.
+
+  top_level_unfold reducible; top_level_unfold reduces_to; steps.
+  eapply star_backstep_reducible; try apply evaluate_select; eauto;
+    repeat step || rewrite pfv_select || list_utils || rewrite substitute_tree in * ||
+           apply wf_select || apply is_erased_term_select ||
+           (rewrite substitute_nothing5 by (steps; eapply reducible_val_fv; eauto; steps));
+    try solve [ eapply reducible_val_fv; eauto; steps ];
+    try solve [ eapply reducible_val_wf; eauto; steps ];
+    try solve [ eapply reducible_values_erased; eauto; steps ];
+    t_closer.
+
+  apply reducible_value_expr; repeat step || list_utils2;
+    eauto using select_type.
+Qed.
+
+
+(** prefix specifies for two sequences of selections whether the first is a prefix of the second *)
+(** prefix: T_key -> T_key -> Prop *)
+Parameter prefix: tree -> tree -> Prop.
+
+(** Finally, `update` takes a tree, a key `k`, another tree, and copies the latter in the first *)
+(** tree at at position `k` *)
+(** update: T_tree -> T_key -> T_tree -> T_tree *)
+Parameter update: tree -> tree -> tree -> tree.
+
+Axiom update_type:
+  forall old_tree key tree,
+    [ old_tree : T_tree ]v ->
+    [ key : T_key ]v ->
+    [ tree : T_tree ]v ->
+    [ update old_tree key tree : T_tree ]v.
+
+Axiom wf_update:
+  forall k t1 t2 t3,
+    wf t1 k ->
+    wf t2 k ->
+    wf t3 k ->
+    wf (update t1 t2 t3) k.
+
+Axiom open_update:
+  forall t1 t2 t3 k rep,
+    open k (update t1 t2 t3) rep =
+    update (open k t1 rep) (open k t2 rep) (open k t3 rep).
+
+Axiom psubstitute_update:
+  forall t1 t2 t3 l tag,
+    psubstitute (update t1 t2 t3) l tag =
+    update (psubstitute t1 l tag) (psubstitute t2 l tag) (psubstitute t3 l tag).
+
+Axiom pfv_update:
+  forall t1 t2 t3 tag,
+    pfv (update t1 t2 t3) tag = pfv t1 tag ++ pfv t2 tag ++ pfv t3 tag.
+
+Axiom is_erased_term_update:
+  forall t1 t2 t3,
+    is_erased_term t1 ->
+    is_erased_term t2 ->
+    is_erased_term t3 ->
+    is_erased_term (update t1 t2 t3).
+
+
+(** Updates that happen on selections which are not prefixes of another are commutative *)
+Axiom update_commutative:
+  forall key1 key2 old_tree tree1 tree2,
+    [ key1 : T_key ]v ->
+    [ key2 : T_key ]v ->
+    [ tree1 : T_tree ]v ->
+    [ tree2 : T_tree ]v ->
+    [ old_tree : T_tree ]v ->
+    ~ prefix key1 key2 ->
+    ~ prefix key2 key1 ->
+      update (update old_tree key2 tree2) key1 tree1 =
+      update (update old_tree key1 tree1) key2 tree2.
+
+(** Selecting at a key after an update gives back the replaced tree *)
+Axiom select_update:
+  forall key old_tree tree,
+    select key (update old_tree key tree) = tree.
+
+Hint Resolve pfv_update: pfv.
+Hint Resolve wf_update: wf.
+Hint Resolve is_erased_term_update: erased.
